Reflection/Util/Sum.lean
@@ -4,7 +4,7 @@ import Mathlib.Tactic.Ring
 
 /-- "Big sum" operator $Σ_{i = lower}^{upper - 1} f(i)$.\
   **Note the exclusive upper bound `-1`!** -/
-@[aesop unsafe] def sum (lower upper : Nat) (f : (x : Nat) -> x >= lower ∧ x < upper -> Nat) : Nat :=
+@[aesop unsafe] abbrev sum (lower upper : Nat) (f : (x : Nat) -> x >= lower ∧ x < upper -> Nat) : Nat :=
   if h : lower < upper then
     (f lower (by simp_all only [ge_iff_le, le_refl, and_self]))
     + sum (lower + 1) upper (fun x hx => f x (by omega))
@@ -17,7 +17,7 @@ example : sum 2 4 (fun i _ => 10 + i) = (10 + 2) + (10 + 3) := rfl
 
 @[aesop unsafe] theorem sum_begin (h : lower < upper)
   : sum lower upper f = f lower (by omega) + sum (lower + 1) upper (fun x hx => f x (by omega))
-  := by rw [sum]; simp_all only [↓reduceDite]
+  := by rw [sum]; simp_all only [↓reduceDIte]
 @[simp] theorem sum_zero : sum n n f = 0 := by rw [sum]; simp
 @[aesop unsafe] theorem sum_end (h : lower <= upper)
   : sum lower (upper + 1) f = sum lower upper (fun x hx => f x (by omega)) + f upper (by omega)
